LambdaCalculusAndTypeSoundness: untyped lambda calculus semantics, two ways

LambdaCalculusAndTypeSoundness.v
@@ -5,517 +5,725 @@
 
 Require Import Frap.
 
-(* Expression syntax *)
-Inductive exp : Set :=
-| Var (x : var)
-| Const (n : nat)
-| Plus (e1 e2 : exp)
-| Abs (x : var) (e1 : exp)
-| App (e1 e2 : exp).
-
-(* Values (final results of evaluation) *)
-Inductive value : exp -> Prop :=
-| VConst : forall n, value (Const n)
-| VAbs : forall x e1, value (Abs x e1).
-
-(* Substitution (not applicable when [e1] isn't closed, to avoid some complexity
- * that we don't need) *)
-Fixpoint subst (e1 : exp) (x : string) (e2 : exp) : exp :=
-  match e2 with
-    | Var y => if y ==v x then e1 else Var y
-    | Const n => Const n
-    | Plus e2' e2'' => Plus (subst e1 x e2') (subst e1 x e2'')
-    | Abs y e2' => Abs y (if y ==v x then e2' else subst e1 x e2')
-    | App e2' e2'' => App (subst e1 x e2') (subst e1 x e2'')
-  end.
-
-(* Evaluation contexts *)
-Inductive context : Set :=
-| Hole : context
-| Plus1 : context -> exp -> context
-| Plus2 : exp -> context -> context
-| App1 : context -> exp -> context
-| App2 : exp -> context -> context.
-
-(* Plugging an expression into a context *)
-Inductive plug : context -> exp -> exp -> Prop :=
-| PlugHole : forall e, plug Hole e e
-| PlugPlus1 : forall e e' C e2,
-  plug C e e'
-  -> plug (Plus1 C e2) e (Plus e' e2)
-| PlugPlus2 : forall e e' v1 C,
-  value v1
-  -> plug C e e'
-  -> plug (Plus2 v1 C) e (Plus v1 e')
-| PlugApp1 : forall e e' C e2,
-  plug C e e'
-  -> plug (App1 C e2) e (App e' e2)
-| PlugApp2 : forall e e' v1 C,
-  value v1
-  -> plug C e e'
-  -> plug (App2 v1 C) e (App v1 e').
-
-(* Small-step, call-by-value evaluation, using our evaluation contexts *)
-
-(* First: the primitive reductions *)
-Inductive step0 : exp -> exp -> Prop :=
-| Beta : forall x e v,
-  value v
-  -> step0 (App (Abs x e) v) (subst v x e)
-| Add : forall n1 n2,
-  step0 (Plus (Const n1) (Const n2)) (Const (n1 + n2)).
-
-(* Then: running them in context *)
-Inductive step : exp -> exp -> Prop :=
-| StepRule : forall C e1 e2 e1' e2',
-  plug C e1 e1'
-  -> plug C e2 e2'
-  -> step0 e1 e2
-  -> step e1' e2'.
-
-(* It's easy to wrap everything as a transition system. *)
-Definition trsys_of (e : exp) := {|
-  Initial := {e};
-  Step := step
-|}.
-
-
-(* Syntax of types *)
-Inductive type : Set :=
-| Nat
-| Fun (dom ran : type).
-
-(* Our typing judgment uses *typing contexts* (not to be confused with
- * evaluation contexts) to map free variables to their types. *)
-Inductive hasty : fmap var type -> exp -> type -> Prop :=
-| HtVar : forall G x t,
-  G $? x = Some t
-  -> hasty G (Var x) t
-| HtConst : forall G n,
-  hasty G (Const n) Nat
-| HtPlus : forall G e1 e2,
-  hasty G e1 Nat
-  -> hasty G e2 Nat
-  -> hasty G (Plus e1 e2) Nat
-| HtAbs : forall G x e1 t1 t2,
-  hasty (G $+ (x, t1)) e1 t2
-  -> hasty G (Abs x e1) (Fun t1 t2)
-| HtApp : forall G e1 e2 t1 t2,
-  hasty G e1 (Fun t1 t2)
-  -> hasty G e2 t1
-  -> hasty G (App e1 e2) t2.
-
-Hint Constructors value plug step0 step hasty.
-
-
-(** * Let's prove type soundness first without much automation. *)
-
-(* Now we're ready for the first of the two key properties, to show that "has
- * type t in the empty typing context" is an invariant. *)
-Lemma progress : forall e t,
-  hasty $0 e t
-  -> value e
-  \/ (exists e' : exp, step e e').
-Proof.
-  induct 1; simplify; try equality.
-
-  left.
-  constructor.
-
-  propositional.
-
-  right.
-  invert H1; invert H.
-  invert H2; invert H0.
-  exists (Const (n + n0)).
-  eapply StepRule with (C := Hole).
-  eauto.
-  eauto.
-  constructor.
-
-  invert H2.
-  right.
-  invert H3.
-  exists (Plus e1 x).
-  eapply StepRule with (C := Plus2 e1 C).
-  eauto.
-  eauto.
-  assumption.
-
-  invert H1.
-  invert H3.
-  right.
-  exists (Plus x e2).
-  eapply StepRule with (C := Plus1 C e2).
-  eauto.
-  eauto.
-  assumption.
-
-  invert H1.
-  invert H3.
-  right.
-  exists (Plus x e2).
-  eapply StepRule with (C := Plus1 C e2).
-  eauto.
-  eauto.
-  assumption.
-
-  left.
-  constructor.
-
-  propositional.
-  
-  right.
-  invert H1; invert H.
-  exists (subst e2 x e0).
-  eapply StepRule with (C := Hole).
-  eauto.
-  eauto.
-  constructor.
-  assumption.
-
-  invert H2.
-  right.
-  invert H3.
-  exists (App e1 x).
-  eapply StepRule with (C := App2 e1 C).
-  eauto.
-  eauto.
-  assumption.
-
-  invert H1.
-  invert H3.
-  right.
-  exists (App x e2).
-  eapply StepRule with (C := App1 C e2).
-  eauto.
-  eauto.
-  assumption.
-
-  invert H1.
-  invert H3.
-  right.
-  exists (App x e2).
-  eapply StepRule with (C := App1 C e2).
-  eauto.
-  eauto.
-  assumption.
-Qed.
-
-(* Inclusion between typing contexts is preserved by adding the same new mapping
- * to both. *)
-Lemma weakening_override : forall (G G' : fmap var type) x t,
-  (forall x' t', G $? x' = Some t' -> G' $? x' = Some t')
-  -> (forall x' t', G $+ (x, t) $? x' = Some t'
-                    -> G' $+ (x, t) $? x' = Some t').
-Proof.
-  simplify.
-  cases (x ==v x'); simplify; eauto.
-Qed.
-
-(** Raising a typing derivation to a larger typing context *)
-Lemma weakening : forall G e t,
-  hasty G e t
-  -> forall G', (forall x t, G $? x = Some t -> G' $? x = Some t)
-    -> hasty G' e t.
-Proof.
-  induct 1; simplify.
-
-  constructor.
-  apply H0.
-  assumption.
-
-  constructor.
-
-  constructor.
-  apply IHhasty1.
-  assumption.
-  apply IHhasty2.
-  assumption.
-
-  constructor.
-  apply IHhasty.
-  apply weakening_override.
-  assumption.
-
-  econstructor.
-  apply IHhasty1.
-  assumption.
-  apply IHhasty2.
-  assumption.
-Qed.
-
-(* Replacing a variable with a properly typed term preserves typing. *)
-Lemma substitution : forall G x t' e t e',
-  hasty (G $+ (x, t')) e t
-  -> hasty $0 e' t'
-  -> hasty G (subst e' x e) t.
-Proof.
-  induct 1; simplify.
-
-  cases (x0 ==v x).
-
-  simplify.
-  invert H.
-  eapply weakening.
-  eassumption.
-  simplify.
-  equality.
-
-  simplify.
-  constructor.
-  assumption.
-
-  constructor.
-
-  constructor.
-  apply IHhasty1.
-  assumption.
-  apply IHhasty2.
-  assumption.
-
-  cases (x0 ==v x).
-
-  constructor.
-  eapply weakening.
-  eassumption.
-  simplify.
-  cases (x0 ==v x1).
-
-  simplify.
-  assumption.
-
-  simplify.
-  assumption.
-
-  constructor.
-  eapply IHhasty.
-  maps_equal.
-  assumption.
-
-  econstructor.
-  apply IHhasty1.
-  assumption.
-  apply IHhasty2.
-  assumption.
-Qed.
-
-(* We're almost ready for the main preservation property.  Let's prove it first
- * for the more basic [step0] relation. *)
-Lemma preservation0 : forall e1 e2,
-  step0 e1 e2
-  -> forall t, hasty $0 e1 t
-    -> hasty $0 e2 t.
-Proof.
-  invert 1; simplify.
-
-  invert H.
-  invert H4.
-  eapply substitution.
-  eassumption.
-  assumption.
-  
-  invert H.
-  constructor.
-Qed.
-
-(* We also need this key property, essentially saying that, if [e1] and [e2] are
- * "type-equivalent," then they remain "type-equivalent" after wrapping the same
- * context around both. *)
-Lemma generalize_plug : forall e1 C e1',
-  plug C e1 e1'
-  -> forall e2 e2', plug C e2 e2'
-    -> (forall t, hasty $0 e1 t -> hasty $0 e2 t)
-    -> (forall t, hasty $0 e1' t -> hasty $0 e2' t).
-Proof.
-  induct 1; simplify.
-
-  invert H.
-  apply H0.
-  assumption.
-
-  invert H0.
-  invert H2.
-  constructor.
-  eapply IHplug.
-  eassumption.
-  assumption.
-  assumption.
-  assumption.
-
-  invert H1.
-  invert H3.
-  constructor.
-  assumption.
-  eapply IHplug.
-  eassumption.
-  assumption.
-  assumption.
-
-  invert H0.
-  invert H2.
-  econstructor.
-  eapply IHplug.
-  eassumption.
-  assumption.
-  eassumption.
-  assumption.
-
-  invert H1.
-  invert H3.
-  econstructor.
-  eassumption.
-  eapply IHplug.
-  eassumption.
-  assumption.
-  eassumption.
-Qed.
-
-(* OK, now we're almost done. *)
-Lemma preservation : forall e1 e2,
-  step e1 e2
-  -> forall t, hasty $0 e1 t
-    -> hasty $0 e2 t.
-Proof.
-  invert 1; simplify.
-
-  eapply generalize_plug with (e1' := e1).
-  eassumption.
-  eassumption.
-  simplify.
-  eapply preservation0.
-  eassumption.
-  assumption.
-  assumption.
-Qed.
-
-(* Now watch this!  Though the syntactic approach to type soundness is usually
- * presented from scratch as a proof technique, it turns out that the two key
- * properties, progress and preservation, are just instances of the same methods
- * we've been applying all along with invariants of transition systems! *)
-Theorem safety : forall e t, hasty $0 e t
-  -> invariantFor (trsys_of e)
-                  (fun e' => value e'
-                             \/ exists e'', step e' e'').
-Proof.
-  simplify.
-
-  (* Step 1: strengthen the invariant.  In particular, the typing relation is
-   * exactly the right stronger invariant!  Our progress theorem proves the
-   * required invariant inclusion. *)
-  apply invariant_weaken with (invariant1 := fun e' => hasty $0 e' t).
-
-  (* Step 2: apply invariant induction, whose induction step turns out to match
-   * our preservation theorem exactly! *)
-  apply invariant_induction; simplify.
-  equality.
-
-  eapply preservation.
-  eassumption.
-  assumption.
-
-  simplify.
-  eapply progress.
-  eassumption.
-Qed.
-
-
-(** * Let's do that again with more automation. *)
-
-Ltac t0 := match goal with
-           | [ H : ex _ |- _ ] => destruct H
-           | [ H : _ /\ _ |- _ ] => destruct H
-           | [ |- context[?x ==v ?y] ] => destruct (x ==v y)
-           | [ H : Some _ = Some _ |- _ ] => invert H
-
-           | [ H : step _ _ |- _ ] => invert H
-           | [ H : step0 _ _ |- _ ] => invert1 H
-           | [ H : hasty _ ?e _, H' : value ?e |- _ ] => invert H'; invert H
-           | [ H : hasty _ _ _ |- _ ] => invert1 H
-           | [ H : plug _ _ _ |- _ ] => invert1 H
-           end; subst.
-
-Ltac t := simplify; propositional; repeat (t0; simplify); try congruence; eauto 6.
-
-Lemma progress_snazzy : forall e t,
-  hasty $0 e t
-  -> value e
-  \/ (exists e' : exp, step e e').
-Proof.
-  induct 1; t.
-Qed.
-
-Hint Resolve weakening_override.
-
-Lemma weakening_snazzy : forall G e t,
-  hasty G e t
-  -> forall G', (forall x t, G $? x = Some t -> G' $? x = Some t)
-    -> hasty G' e t.
-Proof.
-  induct 1; t.
-Qed.
-
-Hint Resolve weakening_snazzy.
-
-(* Replacing a typing context with an equal one has no effect (useful to guide
- * proof search). *)
-Lemma hasty_change : forall G e t,
-  hasty G e t
-  -> forall G', G' = G
-    -> hasty G' e t.
-Proof.
-  t.
-Qed.
-
-Hint Resolve hasty_change.
-
-Lemma substitution_snazzy : forall G x t' e t e',
-  hasty (G $+ (x, t')) e t
-  -> hasty $0 e' t'
-  -> hasty G (subst e' x e) t.
-Proof.
-  induct 1; t.
-Qed.
-
-Hint Resolve substitution_snazzy.
-
-Lemma preservation0_snazzy : forall e1 e2,
-  step0 e1 e2
-  -> forall t, hasty $0 e1 t
-    -> hasty $0 e2 t.
-Proof.
-  invert 1; t.
-Qed.
-
-Hint Resolve preservation0_snazzy.
-
-Lemma generalize_plug_snazzy : forall e1 C e1',
-  plug C e1 e1'
-  -> forall e2 e2', plug C e2 e2'
-    -> (forall t, hasty $0 e1 t -> hasty $0 e2 t)
-    -> (forall t, hasty $0 e1' t -> hasty $0 e2' t).
-Proof.
-  induct 1; t.
-Qed.
-
-Hint Resolve generalize_plug_snazzy.
-
-Lemma preservation_snazzy : forall e1 e2,
-  step e1 e2
-  -> forall t, hasty $0 e1 t
-    -> hasty $0 e2 t.
-Proof.
-  invert 1; t.
-Qed.
-
-Hint Resolve progress_snazzy preservation_snazzy.
-
-Theorem safety_snazzy : forall e t, hasty $0 e t
-  -> invariantFor (trsys_of e)
-                  (fun e' => value e'
-                             \/ exists e'', step e' e'').
-Proof.
-  simplify.
-  apply invariant_weaken with (invariant1 := fun e' => hasty $0 e' t); eauto.
-  apply invariant_induction; simplify; eauto; equality.
-Qed.
+Module Ulc.
+  Inductive exp : Set :=
+  | Var : var -> exp
+  | Abs : var -> exp -> exp
+  | App : exp -> exp -> exp.
+
+  Fixpoint subst (rep : exp) (x : string) (e : exp) : exp :=
+    match e with
+    | Var y => if string_dec y x then rep else Var y
+    | Abs y e1 => Abs y (if string_dec y x then e1 else subst rep x e1)
+    | App e1 e2 => App (subst rep x e1) (subst rep x e2)
+    end.
+
+
+  (** * Big-step semantics *)
+
+  (** This is the most straightforward way to give semantics to lambda terms:
+    * We evaluate any closed term into a value (that is, an [Abs]). *)
+  Inductive eval : exp -> exp -> Prop :=
+  | BigAbs : forall x e,
+    eval (Abs x e) (Abs x e)
+  | BigApp : forall e1 x e1' e2 v2 v,
+    eval e1 (Abs x e1')
+    -> eval e2 v2
+    -> eval (subst v2 x e1') v
+    -> eval (App e1 e2) v.
+
+  (** Note that we omit a [Var] case, since variable terms can't be *closed*. *)
+
+
+  (** Which terms are values, that is, final results of execution? *)
+  Inductive value : exp -> Prop :=
+  | Value : forall x e, value (Abs x e).
+  (** We're cheating a bit here, *assuming* that the term is also closed. *)
+
+  Hint Constructors eval value.
+
+  (** Actually, let's prove that [eval] only produces values. *)
+  Theorem eval_value : forall e v,
+    eval e v
+    -> value v.
+  Proof.
+    induct 1; eauto.
+  Qed.
+
+
+  (** * Small-step semantics with evaluation contexts *)
+
+  Inductive context : Set :=
+  | Hole : context
+  | App1 : context -> exp -> context
+  | App2 : exp -> context -> context.
+
+  Inductive plug : context -> exp -> exp -> Prop :=
+  | PlugHole : forall e,
+    plug Hole e e
+  | PlugApp1 : forall c e1 e2 e,
+    plug c e1 e
+    -> plug (App1 c e2) e1 (App e e2)
+  | PlugApp2 : forall c e1 e2 e,
+    value e1
+    -> plug c e2 e
+    -> plug (App2 e1 c) e2 (App e1 e).
+  (* Subtle point: the [value] hypothesis right above enforces a well-formedness
+   * condition on contexts that may actually be plugged.  We don't allow
+   * skipping over a lefthand subterm of an application when that term has
+   * evaluation work left to do.  This condition is the essence of
+   * *call-by-value* instead of other evaluation strategies.  Details are
+   * largely beyond our scope here. *)
+
+  Inductive step : exp -> exp -> Prop :=
+  | ContextBeta : forall c x e v e1 e2,
+    value v
+    -> plug c (App (Abs x e) v) e1
+    -> plug c (subst v x e) e2
+    -> step e1 e2.
+
+  Hint Constructors plug step.
+
+  (** We can move directly to establishing inclusion from basic small steps to contextual small steps. *)
+
+  Theorem value_eval : forall v,
+    value v
+    -> eval v v.
+  Proof.
+    invert 1; eauto.
+  Qed.
+
+  Hint Resolve value_eval.
+
+  Lemma step_eval'' : forall v c x e e1 e2 v0,
+    value v
+    -> plug c (App (Abs x e) v) e1
+    -> plug c (subst v x e) e2
+    -> eval e2 v0
+    -> eval e1 v0.
+  Proof.
+    induct c; invert 2; invert 1; simplify; eauto.
+    invert H0; eauto.
+    invert H0; eauto.
+  Qed.
+
+  Hint Resolve step_eval''.
+
+  Lemma step_eval' : forall e1 e2,
+    step e1 e2
+    -> forall v, eval e2 v
+      -> eval e1 v.
+  Proof.
+    invert 1; simplify; eauto.
+  Qed.
+
+  Hint Resolve step_eval'.
+
+  Theorem step_eval : forall e v,
+    step^* e v
+    -> value v
+    -> eval e v.
+  Proof.
+    induct 1; eauto.
+  Qed.
+
+  Lemma plug_functional : forall C e e1,
+      plug C e e1
+      -> forall e2, plug C e e2
+                    -> e1 = e2.
+  Proof.
+    induct 1; invert 1; simplify; try f_equal; eauto.
+  Qed.
+
+  Lemma plug_mirror : forall C e e', plug C e e'
+    -> forall e1, exists e1', plug C e1 e1'.
+  Proof.
+    induct 1; simplify; eauto.
+
+    specialize (IHplug e0); first_order; eauto.
+
+    specialize (IHplug e0); first_order; eauto.
+  Qed.    
+
+  Fixpoint compose (C1 C2 : context) : context :=
+    match C2 with
+    | Hole => C1
+    | App1 C2' e => App1 (compose C1 C2') e
+    | App2 v C2' => App2 v (compose C1 C2')
+    end.
+
+  Lemma compose_ok : forall C1 C2 e1 e2 e3,
+      plug C1 e1 e2
+      -> plug C2 e2 e3
+      -> plug (compose C1 C2) e1 e3.
+  Proof.
+    induct 2; simplify; eauto.
+  Qed.
+
+  Hint Resolve compose_ok.
+
+  Lemma step_plug : forall e1 e2,
+    step e1 e2
+    -> forall C e1' e2', plug C e1 e1'
+                         -> plug C e2 e2'
+                         -> step e1' e2'.
+  Proof.
+    invert 1; simplify; eauto.
+  Qed.
+
+  Lemma stepStar_plug : forall e1 e2,
+    step^* e1 e2
+    -> forall C e1' e2', plug C e1 e1'
+                         -> plug C e2 e2'
+                         -> step^* e1' e2'.
+  Proof.
+    induct 1; simplify.
+
+    assert (e1' = e2') by (eapply plug_functional; eassumption).
+    subst.
+    constructor.
+
+    assert (exists y', plug C y y') by eauto using plug_mirror.
+    invert H3.
+    eapply step_plug in H.
+    econstructor.
+    eassumption.
+    eapply IHtrc.
+    eassumption.
+    assumption.
+    eassumption.
+    assumption.
+  Qed.
+
+  Hint Resolve stepStar_plug eval_value.
+
+  Theorem eval_step : forall e v,
+    eval e v
+    -> step^* e v.
+  Proof.
+    induct 1; eauto.
+
+    eapply trc_trans.
+    eapply stepStar_plug with (e1 := e1) (e2 := Abs x e1') (C := App1 Hole e2); eauto.
+    eapply trc_trans.
+    eapply stepStar_plug with (e1 := e2) (e2 := v2) (C := App2 (Abs x e1') Hole); eauto.
+    eauto.
+  Qed.
+End Ulc.
+
+Module Stlc.
+  (* Expression syntax *)
+  Inductive exp : Set :=
+  | Var (x : var)
+  | Const (n : nat)
+  | Plus (e1 e2 : exp)
+  | Abs (x : var) (e1 : exp)
+  | App (e1 e2 : exp).
+
+  (* Values (final results of evaluation) *)
+  Inductive value : exp -> Prop :=
+  | VConst : forall n, value (Const n)
+  | VAbs : forall x e1, value (Abs x e1).
+
+  (* Substitution (not applicable when [e1] isn't closed, to avoid some complexity
+   * that we don't need) *)
+  Fixpoint subst (e1 : exp) (x : string) (e2 : exp) : exp :=
+    match e2 with
+      | Var y => if y ==v x then e1 else Var y
+      | Const n => Const n
+      | Plus e2' e2'' => Plus (subst e1 x e2') (subst e1 x e2'')
+      | Abs y e2' => Abs y (if y ==v x then e2' else subst e1 x e2')
+      | App e2' e2'' => App (subst e1 x e2') (subst e1 x e2'')
+    end.
+
+  (* Evaluation contexts *)
+  Inductive context : Set :=
+  | Hole : context
+  | Plus1 : context -> exp -> context
+  | Plus2 : exp -> context -> context
+  | App1 : context -> exp -> context
+  | App2 : exp -> context -> context.
+
+  (* Plugging an expression into a context *)
+  Inductive plug : context -> exp -> exp -> Prop :=
+  | PlugHole : forall e, plug Hole e e
+  | PlugPlus1 : forall e e' C e2,
+    plug C e e'
+    -> plug (Plus1 C e2) e (Plus e' e2)
+  | PlugPlus2 : forall e e' v1 C,
+    value v1
+    -> plug C e e'
+    -> plug (Plus2 v1 C) e (Plus v1 e')
+  | PlugApp1 : forall e e' C e2,
+    plug C e e'
+    -> plug (App1 C e2) e (App e' e2)
+  | PlugApp2 : forall e e' v1 C,
+    value v1
+    -> plug C e e'
+    -> plug (App2 v1 C) e (App v1 e').
+
+  (* Small-step, call-by-value evaluation, using our evaluation contexts *)
+
+  (* First: the primitive reductions *)
+  Inductive step0 : exp -> exp -> Prop :=
+  | Beta : forall x e v,
+    value v
+    -> step0 (App (Abs x e) v) (subst v x e)
+  | Add : forall n1 n2,
+    step0 (Plus (Const n1) (Const n2)) (Const (n1 + n2)).
+
+  (* Then: running them in context *)
+  Inductive step : exp -> exp -> Prop :=
+  | StepRule : forall C e1 e2 e1' e2',
+    plug C e1 e1'
+    -> plug C e2 e2'
+    -> step0 e1 e2
+    -> step e1' e2'.
+
+  (* It's easy to wrap everything as a transition system. *)
+  Definition trsys_of (e : exp) := {|
+    Initial := {e};
+    Step := step
+  |}.
+
+
+  (* Syntax of types *)
+  Inductive type : Set :=
+  | Nat
+  | Fun (dom ran : type).
+
+  (* Our typing judgment uses *typing contexts* (not to be confused with
+   * evaluation contexts) to map free variables to their types. *)
+  Inductive hasty : fmap var type -> exp -> type -> Prop :=
+  | HtVar : forall G x t,
+    G $? x = Some t
+    -> hasty G (Var x) t
+  | HtConst : forall G n,
+    hasty G (Const n) Nat
+  | HtPlus : forall G e1 e2,
+    hasty G e1 Nat
+    -> hasty G e2 Nat
+    -> hasty G (Plus e1 e2) Nat
+  | HtAbs : forall G x e1 t1 t2,
+    hasty (G $+ (x, t1)) e1 t2
+    -> hasty G (Abs x e1) (Fun t1 t2)
+  | HtApp : forall G e1 e2 t1 t2,
+    hasty G e1 (Fun t1 t2)
+    -> hasty G e2 t1
+    -> hasty G (App e1 e2) t2.
+
+  Hint Constructors value plug step0 step hasty.
+
+
+  (** * Let's prove type soundness first without much automation. *)
+
+  (* Now we're ready for the first of the two key properties, to show that "has
+   * type t in the empty typing context" is an invariant. *)
+  Lemma progress : forall e t,
+    hasty $0 e t
+    -> value e
+    \/ (exists e' : exp, step e e').
+  Proof.
+    induct 1; simplify; try equality.
+
+    left.
+    constructor.
+
+    propositional.
+
+    right.
+    invert H1; invert H.
+    invert H2; invert H0.
+    exists (Const (n + n0)).
+    eapply StepRule with (C := Hole).
+    eauto.
+    eauto.
+    constructor.
+
+    invert H2.
+    right.
+    invert H3.
+    exists (Plus e1 x).
+    eapply StepRule with (C := Plus2 e1 C).
+    eauto.
+    eauto.
+    assumption.
+
+    invert H1.
+    invert H3.
+    right.
+    exists (Plus x e2).
+    eapply StepRule with (C := Plus1 C e2).
+    eauto.
+    eauto.
+    assumption.
+
+    invert H1.
+    invert H3.
+    right.
+    exists (Plus x e2).
+    eapply StepRule with (C := Plus1 C e2).
+    eauto.
+    eauto.
+    assumption.
+
+    left.
+    constructor.
+
+    propositional.
+
+    right.
+    invert H1; invert H.
+    exists (subst e2 x e0).
+    eapply StepRule with (C := Hole).
+    eauto.
+    eauto.
+    constructor.
+    assumption.
+
+    invert H2.
+    right.
+    invert H3.
+    exists (App e1 x).
+    eapply StepRule with (C := App2 e1 C).
+    eauto.
+    eauto.
+    assumption.
+
+    invert H1.
+    invert H3.
+    right.
+    exists (App x e2).
+    eapply StepRule with (C := App1 C e2).
+    eauto.
+    eauto.
+    assumption.
+
+    invert H1.
+    invert H3.
+    right.
+    exists (App x e2).
+    eapply StepRule with (C := App1 C e2).
+    eauto.
+    eauto.
+    assumption.
+  Qed.
+
+  (* Inclusion between typing contexts is preserved by adding the same new mapping
+   * to both. *)
+  Lemma weakening_override : forall (G G' : fmap var type) x t,
+    (forall x' t', G $? x' = Some t' -> G' $? x' = Some t')
+    -> (forall x' t', G $+ (x, t) $? x' = Some t'
+                      -> G' $+ (x, t) $? x' = Some t').
+  Proof.
+    simplify.
+    cases (x ==v x'); simplify; eauto.
+  Qed.
+
+  (** Raising a typing derivation to a larger typing context *)
+  Lemma weakening : forall G e t,
+    hasty G e t
+    -> forall G', (forall x t, G $? x = Some t -> G' $? x = Some t)
+      -> hasty G' e t.
+  Proof.
+    induct 1; simplify.
+
+    constructor.
+    apply H0.
+    assumption.
+
+    constructor.
+
+    constructor.
+    apply IHhasty1.
+    assumption.
+    apply IHhasty2.
+    assumption.
+
+    constructor.
+    apply IHhasty.
+    apply weakening_override.
+    assumption.
+
+    econstructor.
+    apply IHhasty1.
+    assumption.
+    apply IHhasty2.
+    assumption.
+  Qed.
+
+  (* Replacing a variable with a properly typed term preserves typing. *)
+  Lemma substitution : forall G x t' e t e',
+    hasty (G $+ (x, t')) e t
+    -> hasty $0 e' t'
+    -> hasty G (subst e' x e) t.
+  Proof.
+    induct 1; simplify.
+
+    cases (x0 ==v x).
+
+    simplify.
+    invert H.
+    eapply weakening.
+    eassumption.
+    simplify.
+    equality.
+
+    simplify.
+    constructor.
+    assumption.
+
+    constructor.
+
+    constructor.
+    apply IHhasty1.
+    assumption.
+    apply IHhasty2.
+    assumption.
+
+    cases (x0 ==v x).
+
+    constructor.
+    eapply weakening.
+    eassumption.
+    simplify.
+    cases (x0 ==v x1).
+
+    simplify.
+    assumption.
+
+    simplify.
+    assumption.
+
+    constructor.
+    eapply IHhasty.
+    maps_equal.
+    assumption.
+
+    econstructor.
+    apply IHhasty1.
+    assumption.
+    apply IHhasty2.
+    assumption.
+  Qed.
+
+  (* We're almost ready for the main preservation property.  Let's prove it first
+   * for the more basic [step0] relation. *)
+  Lemma preservation0 : forall e1 e2,
+    step0 e1 e2
+    -> forall t, hasty $0 e1 t
+      -> hasty $0 e2 t.
+  Proof.
+    invert 1; simplify.
+
+    invert H.
+    invert H4.
+    eapply substitution.
+    eassumption.
+    assumption.
+
+    invert H.
+    constructor.
+  Qed.
+
+  (* We also need this key property, essentially saying that, if [e1] and [e2] are
+   * "type-equivalent," then they remain "type-equivalent" after wrapping the same
+   * context around both. *)
+  Lemma generalize_plug : forall e1 C e1',
+    plug C e1 e1'
+    -> forall e2 e2', plug C e2 e2'
+      -> (forall t, hasty $0 e1 t -> hasty $0 e2 t)
+      -> (forall t, hasty $0 e1' t -> hasty $0 e2' t).
+  Proof.
+    induct 1; simplify.
+
+    invert H.
+    apply H0.
+    assumption.
+
+    invert H0.
+    invert H2.
+    constructor.
+    eapply IHplug.
+    eassumption.
+    assumption.
+    assumption.
+    assumption.
+
+    invert H1.
+    invert H3.
+    constructor.
+    assumption.
+    eapply IHplug.
+    eassumption.
+    assumption.
+    assumption.
+
+    invert H0.
+    invert H2.
+    econstructor.
+    eapply IHplug.
+    eassumption.
+    assumption.
+    eassumption.
+    assumption.
+
+    invert H1.
+    invert H3.
+    econstructor.
+    eassumption.
+    eapply IHplug.
+    eassumption.
+    assumption.
+    eassumption.
+  Qed.
+
+  (* OK, now we're almost done. *)
+  Lemma preservation : forall e1 e2,
+    step e1 e2
+    -> forall t, hasty $0 e1 t
+      -> hasty $0 e2 t.
+  Proof.
+    invert 1; simplify.
+
+    eapply generalize_plug with (e1' := e1).
+    eassumption.
+    eassumption.
+    simplify.
+    eapply preservation0.
+    eassumption.
+    assumption.
+    assumption.
+  Qed.
+
+  (* Now watch this!  Though the syntactic approach to type soundness is usually
+   * presented from scratch as a proof technique, it turns out that the two key
+   * properties, progress and preservation, are just instances of the same methods
+   * we've been applying all along with invariants of transition systems! *)
+  Theorem safety : forall e t, hasty $0 e t
+    -> invariantFor (trsys_of e)
+                    (fun e' => value e'
+                               \/ exists e'', step e' e'').
+  Proof.
+    simplify.
+
+    (* Step 1: strengthen the invariant.  In particular, the typing relation is
+     * exactly the right stronger invariant!  Our progress theorem proves the
+     * required invariant inclusion. *)
+    apply invariant_weaken with (invariant1 := fun e' => hasty $0 e' t).
+
+    (* Step 2: apply invariant induction, whose induction step turns out to match
+     * our preservation theorem exactly! *)
+    apply invariant_induction; simplify.
+    equality.
+
+    eapply preservation.
+    eassumption.
+    assumption.
+
+    simplify.
+    eapply progress.
+    eassumption.
+  Qed.
+
+
+  (** * Let's do that again with more automation. *)
+
+  Ltac t0 := match goal with
+             | [ H : ex _ |- _ ] => destruct H
+             | [ H : _ /\ _ |- _ ] => destruct H
+             | [ |- context[?x ==v ?y] ] => destruct (x ==v y)
+             | [ H : Some _ = Some _ |- _ ] => invert H
+
+             | [ H : step _ _ |- _ ] => invert H
+             | [ H : step0 _ _ |- _ ] => invert1 H
+             | [ H : hasty _ ?e _, H' : value ?e |- _ ] => invert H'; invert H
+             | [ H : hasty _ _ _ |- _ ] => invert1 H
+             | [ H : plug _ _ _ |- _ ] => invert1 H
+             end; subst.
+
+  Ltac t := simplify; propositional; repeat (t0; simplify); try congruence; eauto 6.
+
+  Lemma progress_snazzy : forall e t,
+    hasty $0 e t
+    -> value e
+    \/ (exists e' : exp, step e e').
+  Proof.
+    induct 1; t.
+  Qed.
+
+  Hint Resolve weakening_override.
+
+  Lemma weakening_snazzy : forall G e t,
+    hasty G e t
+    -> forall G', (forall x t, G $? x = Some t -> G' $? x = Some t)
+      -> hasty G' e t.
+  Proof.
+    induct 1; t.
+  Qed.
+
+  Hint Resolve weakening_snazzy.
+
+  (* Replacing a typing context with an equal one has no effect (useful to guide
+   * proof search). *)
+  Lemma hasty_change : forall G e t,
+    hasty G e t
+    -> forall G', G' = G
+      -> hasty G' e t.
+  Proof.
+    t.
+  Qed.
+
+  Hint Resolve hasty_change.
+
+  Lemma substitution_snazzy : forall G x t' e t e',
+    hasty (G $+ (x, t')) e t
+    -> hasty $0 e' t'
+    -> hasty G (subst e' x e) t.
+  Proof.
+    induct 1; t.
+  Qed.
+
+  Hint Resolve substitution_snazzy.
+
+  Lemma preservation0_snazzy : forall e1 e2,
+    step0 e1 e2
+    -> forall t, hasty $0 e1 t
+      -> hasty $0 e2 t.
+  Proof.
+    invert 1; t.
+  Qed.
+
+  Hint Resolve preservation0_snazzy.
+
+  Lemma generalize_plug_snazzy : forall e1 C e1',
+    plug C e1 e1'
+    -> forall e2 e2', plug C e2 e2'
+      -> (forall t, hasty $0 e1 t -> hasty $0 e2 t)
+      -> (forall t, hasty $0 e1' t -> hasty $0 e2' t).
+  Proof.
+    induct 1; t.
+  Qed.
+
+  Hint Resolve generalize_plug_snazzy.
+
+  Lemma preservation_snazzy : forall e1 e2,
+    step e1 e2
+    -> forall t, hasty $0 e1 t
+      -> hasty $0 e2 t.
+  Proof.
+    invert 1; t.
+  Qed.
+
+  Hint Resolve progress_snazzy preservation_snazzy.
+
+  Theorem safety_snazzy : forall e t, hasty $0 e t
+    -> invariantFor (trsys_of e)
+                    (fun e' => value e'
+                               \/ exists e'', step e' e'').
+  Proof.
+    simplify.
+    apply invariant_weaken with (invariant1 := fun e' => hasty $0 e' t); eauto.
+    apply invariant_induction; simplify; eauto; equality.
+  Qed.
+End Stlc.
